more thoughts on adding constraints to models
Ran into a (probably minor) problem:
A type definition introduces both a new type and some new constants. If
the type is constrained but the constants are not, there is no guarantee
that the default (non-constrained) semantics of the constants will be
suitable for the new (constrained) value of the type. So there will
probably need to be some condition on the constraints, saying that if
you constrain a type, you also have to constrain any constants whose
types include that type.

hol-light/standard/semantics/holConstrainedExtensionScript.sml
@@ -1,5 +1,6 @@
-open HolKernel boolLib bossLib lcsymtacs
-open holExtensionTheory
+open HolKernel boolLib bossLib lcsymtacs miscLib
+open miscTheory finite_mapTheory alistTheory listTheory pairTheory
+open holSyntaxTheory holSemanticsTheory holSemanticsExtraTheory holExtensionTheory
 val _ = new_theory"holConstrainedExtension"
 
 val constrain_assignment_def = Define`
@@ -7,20 +8,80 @@ val constrain_assignment_def = Define`
     λname args. case cs name args of SOME x => x | NONE => f name args`
 
 val constrain_interpretation_def = Define`
-  constrain_interpretation (tycs,tmcs) (δ,γ) =
+  constrain_interpretation (tycs,tmcs) ((δ,γ):'U interpretation) =
     (constrain_assignment tycs δ,
      constrain_assignment tmcs γ)`
 
 (*
 val add_constraints_thm = store_thm("add_constraints_thm",
   ``∀i upd ctxt cs.
+      theory_ok (thyof ctxt) ∧ upd updates ctxt ∧
       i models (thyof (upd::ctxt)) ∧
-      (∀name args. IS_SOME ((FST cs) name args) ⇒ MEM (name,LENGTH args) (types_of_upd upd)) ∧
-      (∀name args. IS_SOME ((SND cs) name args) ⇒ MEM (name,LENGTH args) (consts_of_upd upd)) ∧
+      (∀name args. IS_SOME (FST cs name args) ⇒
+        MEM (name,LENGTH args) (types_of_upd upd) ∧
+        inhabited (THE (FST cs name args))) ∧
+      (∀name args. IS_SOME (SND cs name args) ⇒
+        ∃ty. MEM (name,ty) (consts_of_upd upd) ∧
+             (LENGTH (tyvars ty) = LENGTH args) ∧
+             ∀τ. is_type_valuation τ ∧
+                 (MAP τ (STRING_SORT (tyvars ty)) = args) ⇒
+             (THE (SND cs name args)) <: typesem (constrain_assignment (FST cs) (FST i)) τ ty) ∧
       (∀p. MEM p (axioms_of_upd upd) ⇒
         constrain_interpretation cs i satisfies (sigof (upd::ctxt),[],p))
       ⇒
       (constrain_interpretation cs i) models (thyof (upd::ctxt))``,
+  rw[] >> fs[models_def] >>
+  conj_tac >- (
+    Cases_on`i`>>Cases_on`cs`>>fs[is_interpretation_def,constrain_interpretation_def] >>
+    conj_tac >- (
+      fs[is_type_assignment_def,FEVERY_ALL_FLOOKUP] >> rw[] >>
+      res_tac >> rw[constrain_assignment_def] >>
+      BasicProvers.CASE_TAC >> rw[] >>
+      fs[IS_SOME_EXISTS,PULL_EXISTS] >>
+      res_tac >> metis_tac[] ) >>
+    fs[is_term_assignment_def,FEVERY_ALL_FLOOKUP] >> rw[] >>
+    first_x_assum(fn th => first_assum(strip_assume_tac o MATCH_MP th)) >>
+    first_x_assum(fn th => first_assum(strip_assume_tac o MATCH_MP th)) >>
+    rw[constrain_assignment_def] >>
+    reverse BasicProvers.CASE_TAC >- (
+      fs[IS_SOME_EXISTS,PULL_EXISTS] >>
+      first_x_assum(fn th => first_assum(strip_assume_tac o MATCH_MP th)) >>
+      qpat_assum`FLOOKUP X Y = Z`mp_tac >>
+      simp[FLOOKUP_FUNION] >>
+      BasicProvers.CASE_TAC >- (
+        imp_res_tac ALOOKUP_FAILS >> fs[] ) >>
+      rw[] >>
+      `v = ty` by (
+        fs[Once updates_cases] >> rw[] >> fs[] >>
+        qmatch_assum_abbrev_tac`ALOOKUP al k = SOME v` >>
+        `ALL_DISTINCT (MAP FST al)` by (
+          simp[Abbr`al`,MAP_MAP_o,combinTheory.o_DEF,UNCURRY,ETA_AX] ) >>
+        imp_res_tac ALOOKUP_ALL_DISTINCT_MEM >>
+        fs[Abbr`al`] ) >>
+      rw[] >> res_tac >> fs[constrain_assignment_def]) >>
+    qpat_assum`FLOOKUP X Y = Z`mp_tac >>
+    simp[FLOOKUP_FUNION] >>
+    BasicProvers.CASE_TAC >- (
+      strip_tac >>
+      `type_ok (tysof ctxt) v` by (
+        fs[theory_ok_def] >>
+        first_x_assum match_mp_tac >>
+        simp[IN_FRANGE_FLOOKUP] >>
+        metis_tac[] ) >>
+      qmatch_abbrev_tac`a <: b` >>
+      qmatch_assum_abbrev_tac`a <: c` >>
+      qsuff_tac `b = c` >- rw[] >>
+      unabbrev_all_tac >>
+      match_mp_tac typesem_consts >>
+      first_assum(match_exists_tac o concl) >> simp[] >>
+      simp[type_ok_def] >> rw[FUN_EQ_THM] >>
+      BasicProvers.CASE_TAC >>
+      fs[IS_SOME_EXISTS,PULL_EXISTS] >> res_tac >>
+      fs[Once updates_cases] >> rw[] >> fs[] >> rw[] >>
+      imp_res_tac ALOOKUP_MEM >> fs[MEM_MAP,EXISTS_PROD] >>
+      metis_tac[] ) >>
+    rw[] >>
+    fs[Once updates_cases] >> rw[] >> fs[] >> rw[]
 *)
 
 val _ = export_theory()
